add/sub sca

code/ecdsap256sha2/Hacl.Impl.LowLevel.fst
@@ -203,17 +203,28 @@ val add_carry_u64: cin:uint64 -> x:uint64 -> y:uint64 -> r:lbuffer uint64 (size 
       (let r = Seq.index (as_seq h1 r) 0 in
        v r + v c * pow2 64 == v x + v y + v cin))
 
+(*let add_carry_u64 cin x y result1 =
+  assert(uint_v cin + uint_v x + uint_v y < 2 * pow2 64);
+  let res = x +. y +. cin in
+  let c = (lt_mask res x) &. (u64 1) in
+    lt_mask_lemma res x;
+    logand_lemma (lt_mask res x) (u64 1);
+    assert(if v res < v x then uint_v c == 1 else v c == 0);
+
+  result1.(0ul) <- res;
+  c
+*)
+
 let add_carry_u64 cin x y result1 =
   let res1 = x +. cin in
-  let c = (res1 `lt_mask` cin) &. (u64 1) in
-    logand_lemma (lt_mask res1 cin) (u64 1);
+  let c = logand (lt_mask res1 cin) (u64 1) in
   let res = res1 +. y in
-  let c1 = (res `lt_mask` res1) &. (u64 1) in
-      logand_lemma (lt_mask res res1) (u64 1);
+  let c1 = logand (lt_mask res res1) (u64 1)  in 
   result1.(0ul) <- res;
   c +. c1
 
-val sub_borrow_u64_nCT: cin:uint64 -> x:uint64 -> y:uint64 -> r:lbuffer uint64 (size 1) ->
+
+val sub_borrow_u64: cin:uint64 -> x:uint64 -> y:uint64 -> r:lbuffer uint64 (size 1) ->
   Stack uint64
     (requires fun h -> live h r /\ v cin <= 1)
     (ensures  fun h0 c h1 ->
@@ -221,16 +232,13 @@ val sub_borrow_u64_nCT: cin:uint64 -> x:uint64 -> y:uint64 -> r:lbuffer uint64 (
       (let r = Seq.index (as_seq h1 r) 0 in
        v r - v c * pow2 64 == v x - v y - v cin))
 
-let sub_borrow_u64_nCT cin x y result1 =
-  let res = x -. y -. cin in
-  let c =
-    if eq_u64_nCT cin (u64 1) then
-      if le_u64 x y then u64 1 else u64 0
-    else
-      if lt_u64 x y then u64 1 else u64 0
-  in
+let sub_borrow_u64 cin x y result1 =
+  let res = x -. y -. cin in 
+  let eqlty = eq_mask res x in 
+  let c1 = logand (logor (logand cin eqlty) (logand (gte_mask res x) (lognot eqlty))) (u64 1) in 
+  let c = logand (logor (logand cin eqlty) (gt_mask res x)) (u64 1) in 
   result1.(0ul) <- res;
-  c
+  c1
 
 
 val add4: x: felem -> y: felem -> result: felem -> 
